rules/proof_with_lib.v
@@ -1,0 +1,611 @@
+(*
+
+  Copyright 2014 Cornell University
+  Copyright 2015 Cornell University
+  Copyright 2016 Cornell University
+  Copyright 2017 Cornell University
+
+  This file is part of VPrl (the Verified Nuprl project).
+
+  VPrl is free software: you can redistribute it and/or modify
+  it under the terms of the GNU General Public License as published by
+  the Free Software Foundation, either version 3 of the License, or
+  (at your option) any later version.
+
+  VPrl is distributed in the hope that it will be useful,
+  but WITHOUT ANY WARRANTY; without even the implied warranty of
+  MERCHANTABILITY or FITNESS FOR A PARTICULAR PURPOSE.  See the
+  GNU General Public License for more details.
+
+  You should have received a copy of the GNU General Public License
+  along with VPrl.  If not, see <http://www.gnu.org/licenses/>.
+
+
+  Websites: http://nuprl.org/html/verification/
+            http://nuprl.org/html/Nuprl2Coq
+            https://github.com/vrahli/NuprlInCoq
+
+  Authors: Vincent Rahli
+
+*)
+
+
+Require Export rules_isect.
+Require Export rules_squiggle.
+Require Export rules_squiggle2.
+Require Export rules_squiggle3.
+Require Export rules_squiggle5.
+Require Export rules_squiggle6.
+Require Export rules_squiggle7.
+Require Export rules_false.
+Require Export rules_struct.
+Require Export rules_function.
+
+
+
+(* ===========================================================
+
+  A pre-sequent is a sequent without the extract, which we can
+  only build once a proof is finished
+
+  ============================================================ *)
+
+(* a pre-conclusion is a conclusion without the extract *)
+Inductive pre_conclusion {o} :=
+| pre_concl_ext : forall (ctype : @NTerm o), pre_conclusion
+| pre_concl_typ : forall (ctype : @NTerm o), pre_conclusion.
+
+Definition mk_pre_concl {o} (t : @NTerm o) : pre_conclusion :=
+  pre_concl_ext t.
+
+Definition mk_pre_concleq {o} (t1 t2 T : @NTerm o) : pre_conclusion :=
+  mk_pre_concl (mk_equality t1 t2 T).
+
+Record pre_baresequent {p} :=
+  MkPreBaresequent
+    {
+      pre_hyps  : @barehypotheses p;
+      pre_concl : @pre_conclusion p
+    }.
+
+Definition mk_pre_bseq {o} H (c : @pre_conclusion o) : pre_baresequent :=
+  MkPreBaresequent o H c.
+
+Definition concl2pre {o} (c : @conclusion o) : pre_conclusion :=
+  match c with
+  | concl_ext t _ => pre_concl_ext t
+  | concl_typ t => pre_concl_typ t
+  end.
+
+Definition concl2pre_baresequent {o} (c : @conclusion o) : pre_baresequent :=
+  mk_pre_bseq [] (concl2pre c).
+
+Definition baresequent2pre {o} (s : @baresequent o) : pre_baresequent :=
+  mk_pre_bseq (hyps s) (concl2pre (concl s)).
+
+Definition PreStatement {o} (T : @NTerm o) : pre_baresequent :=
+  mk_pre_bseq [] (mk_pre_concl T).
+
+Definition Statement {o} (T : @NTerm o) (e : NTerm) : baresequent :=
+  mk_baresequent [] (mk_concl T e).
+
+
+
+(* ===========================================================
+
+  Some pre-sequents corresponding to the hypotheses and conclusions
+  of some of our rules
+
+  ============================================================ *)
+
+Definition pre_rule_isect_equality_concl {o} a1 a2 x1 x2 b1 b2 i (H : @bhyps o) :=
+  mk_pre_bseq
+    H
+    (mk_pre_concleq
+       (mk_isect a1 x1 b1)
+       (mk_isect a2 x2 b2)
+       (mk_uni i)).
+
+Definition pre_rule_isect_equality_hyp1 {o} a1 a2 i (H : @bhyps o) :=
+  mk_pre_bseq H (mk_pre_concleq a1 a2 (mk_uni i)).
+
+Definition pre_rule_isect_equality_hyp2 {o} a1 b1 b2 x1 x2 y i (H : @bhyps o) :=
+  mk_pre_bseq
+    (snoc H (mk_hyp y a1))
+    (mk_pre_concleq
+       (subst b1 x1 (mk_var y))
+       (subst b2 x2 (mk_var y))
+       (mk_uni i)).
+
+Definition pre_rule_cequiv_concl {o} a b (H : @bhyps o) :=
+  mk_pre_bseq H (mk_pre_concl (mk_cequiv a b)).
+
+Definition pre_rule_function_elimination_concl {o}
+           (A : @NTerm o) B C f x H J :=
+  mk_pre_bseq
+    (snoc H (mk_hyp f (mk_function A x B)) ++ J)
+    (mk_pre_concl C).
+
+Definition pre_rule_function_elimination_hyp1 {o}
+           (A : @NTerm o) B a f x H J :=
+  mk_pre_bseq
+    (snoc H (mk_hyp f (mk_function A x B)) ++ J)
+    (mk_pre_concl (mk_member a A)).
+
+Definition pre_rule_function_elimination_hyp2 {o}
+           (A : @NTerm o) B C a f x z H J :=
+  mk_pre_bseq
+    (snoc (snoc H (mk_hyp f (mk_function A x B)) ++ J)
+          (mk_hyp z (mk_member (mk_apply (mk_var f) a)
+                               (subst B x a))))
+    (mk_pre_concl C).
+
+Definition pre_rule_approx_refl_concl {o} a (H : @bhyps o) :=
+  mk_pre_bseq H (mk_pre_concl (mk_approx a a)).
+
+Definition pre_rule_cequiv_approx_concl {o} (a b : @NTerm o) H :=
+  mk_pre_bseq H (mk_pre_concl (mk_cequiv a b)).
+
+Definition pre_rule_cequiv_approx_hyp {o} (a b : @NTerm o) H :=
+  mk_pre_bseq H (mk_pre_concl (mk_approx a b)).
+
+Definition pre_rule_approx_eq_concl {o} a1 a2 b1 b2 i (H : @bhyps o) :=
+  mk_pre_bseq
+    H
+    (mk_pre_concleq
+       (mk_approx a1 b1)
+       (mk_approx a2 b2)
+       (mk_uni i)).
+
+Definition pre_rule_eq_base_hyp {o} a1 a2 (H : @bhyps o) :=
+  mk_pre_bseq H (mk_pre_concleq a1 a2 mk_base).
+
+Definition pre_rule_cequiv_eq_concl {o} a1 a2 b1 b2 i (H : @bhyps o) :=
+  mk_pre_bseq
+    H
+    (mk_pre_concleq
+       (mk_cequiv a1 b1)
+       (mk_cequiv a2 b2)
+       (mk_uni i)).
+
+Definition pre_rule_bottom_diverges_concl {o} x (H J : @bhyps o) :=
+  mk_pre_bseq
+    (snoc H (mk_hyp x (mk_halts mk_bottom)) ++ J)
+    (mk_pre_concl mk_false).
+
+Definition pre_rule_cut_concl {o} (H : @bhyps o) C :=
+  mk_pre_bseq H (mk_pre_concl C).
+
+Definition pre_rule_cut_hyp1 {o} (H : @bhyps o) B :=
+  mk_pre_bseq H (mk_pre_concl B).
+
+Definition pre_rule_cut_hyp2 {o} (H : @bhyps o) x B C :=
+  mk_pre_bseq (snoc H (mk_hyp x B)) (mk_pre_concl C).
+
+Definition pre_rule_equal_in_base_concl {o} (a b : @NTerm o) H :=
+  mk_pre_bseq H (mk_pre_concl (mk_equality a b mk_base)).
+
+Definition pre_rule_equal_in_base_hyp1 {o} (a b : @NTerm o) H :=
+  mk_pre_bseq H (mk_pre_concl (mk_cequiv a b)).
+
+Definition pre_rule_equal_in_base_hyp2 {o} (v : NVar) (H : @bhyps o) :=
+  mk_pre_bseq H (mk_pre_concl (mk_member (mk_var v) mk_base)).
+
+Definition pre_rule_equal_in_base_rest {o} (a : @NTerm o) (H : @bhyps o) :=
+  map (fun v => pre_rule_equal_in_base_hyp2 v H)
+      (free_vars a).
+
+Definition pre_rule_cequiv_subst_hyp1 {o} (H : @bhyps o) x C a :=
+  mk_pre_bseq H (mk_pre_concl (subst C x a)).
+
+Definition pre_rule_cequiv_subst_hyp2 {o} (H : @bhyps o) a b :=
+  mk_pre_bseq H (mk_pre_concl (mk_cequiv a b)).
+
+Definition pre_rule_hypothesis_concl {o} (G J : @bhyps o) A x :=
+  mk_pre_bseq (snoc G (mk_hyp x A) ++ J) (mk_pre_concl A).
+
+Definition pre_rule_approx_member_eq_concl {o} a b (H : @bhyps o) :=
+  mk_pre_bseq H (mk_pre_concleq mk_axiom mk_axiom (mk_approx a b)).
+
+Definition pre_rule_approx_member_eq_hyp {o} a b (H : @bhyps o) :=
+  mk_pre_bseq H (mk_pre_concl (mk_approx a b)).
+
+
+
+(* ===========================================================
+
+  Side-checks
+
+  ============================================================ *)
+
+Definition NVin v (vs : list NVar) := memvar v vs = false.
+
+Definition Vin v (vs : list NVar) := memvar v vs = true.
+
+Lemma NVin_iff :
+  forall v vs, NVin v vs <=> !LIn v vs.
+Proof.
+  introv.
+  unfold NVin.
+  rw <- (@assert_memberb NVar eq_var_dec).
+  rw <- not_of_assert; sp.
+Qed.
+
+Lemma Vin_iff :
+  forall v vs, Vin v vs <=> LIn v vs.
+Proof.
+  introv.
+  unfold Vin.
+  rw <- (@assert_memberb NVar eq_var_dec); auto.
+Qed.
+
+
+
+(* ===========================================================
+
+  A proof context is a list of abstractions and a list of proved
+  formulas.
+
+  ============================================================ *)
+
+Record ProofContext {o} :=
+  MkProofContext
+    {
+      PC_lib :> @library o;
+      PC_conclusions : list (@conclusion o);
+    }.
+
+Definition EMPC {o} : @ProofContext o := MkProofContext o [] [].
+
+Definition updLibProofContext {o} (pc : @ProofContext o) (e : library_entry) :=
+  MkProofContext
+    o
+    (e :: PC_lib pc)
+    (PC_conclusions pc).
+
+Definition updConclProofContext {o} (pc : @ProofContext o) (c : conclusion) :=
+  MkProofContext
+    o
+    (PC_lib pc)
+    (c :: PC_conclusions pc).
+
+
+
+(* ===========================================================
+
+  A pre-proof is a tree of proof-steps without the extracts,
+  which we can only build once the proof is finished
+
+  ============================================================ *)
+
+(* We have the library here so that we can unfold abstractions *)
+Inductive pre_proof {o} (ctxt : @ProofContext o) : @pre_baresequent o -> Type :=
+| pre_proof_from_ctxt :
+    forall c,
+      LIn c (@PC_conclusions o ctxt)
+      -> pre_proof ctxt (concl2pre_baresequent c)
+| pre_proof_hole : forall s, pre_proof ctxt s
+| pre_proof_isect_eq :
+    forall a1 a2 b1 b2 x1 x2 y i H,
+      NVin y (vars_hyps H)
+      -> pre_proof ctxt (pre_rule_isect_equality_hyp1 a1 a2 i H)
+      -> pre_proof ctxt (pre_rule_isect_equality_hyp2 a1 b1 b2 x1 x2 y i H)
+      -> pre_proof ctxt (pre_rule_isect_equality_concl a1 a2 x1 x2 b1 b2 i H).
+
+Inductive proof {o} (ctxt : @ProofContext o) : @baresequent o -> Type :=
+| proof_from_ctxt :
+    forall c,
+      LIn c (@PC_conclusions o ctxt)
+      -> proof ctxt (mk_baresequent [] c)
+| proof_isect_eq :
+    forall a1 a2 b1 b2 e1 e2 x1 x2 y i H,
+      NVin y (vars_hyps H)
+      -> proof ctxt (rule_isect_equality2_hyp1 a1 a2 e1 i H)
+      -> proof ctxt (rule_isect_equality2_hyp2 a1 b1 b2 e2 x1 x2 y i H)
+      -> proof ctxt (rule_isect_equality_concl a1 a2 x1 x2 b1 b2 i H).
+
+
+
+(* ===========================================================
+
+  State, i.e.:
+    (1) the list of defined abstractions,
+    (2) the list of proved lemmas,
+    (3) the list of lemmas currently being proved
+
+  ============================================================ *)
+
+Definition LemmaName := opname.
+
+Definition opname2opabs (op : opname) : opabs :=
+  mk_opabs op [] [].
+
+Definition name_not_in_lib {o} (name : LemmaName) (l : @library o) :=
+  !in_lib (opname2opabs name) l.
+
+(* !!MOVE *)
+Lemma soterm2nterm_nterm2soterm {o} :
+  forall (t : @NTerm o), soterm2nterm (nterm2soterm t) = t.
+Proof.
+  nterm_ind t as [v|f ind|op bs ind] Case; simpl; auto.
+  Case "oterm".
+  f_equal.
+  rewrite map_map; unfold compose.
+  apply eq_map_l; introv i.
+  destruct x as [vs t]; simpl.
+  f_equal.
+  eapply ind; eauto.
+Qed.
+Hint Rewrite @soterm2nterm_nterm2soterm : slow.
+
+(* !!MOVE *)
+Lemma injective_fun_var2sovar : injective_fun var2sovar.
+Proof.
+  introv e.
+  destruct a1, a2.
+  unfold var2sovar in e; ginv; auto.
+Qed.
+Hint Resolve injective_fun_var2sovar : slow.
+
+(* !!MOVE *)
+Lemma so_free_vars_nterm2soterm {o} :
+  forall (t : @NTerm o),
+    so_free_vars (nterm2soterm t)
+    = vars2sovars (free_vars t).
+Proof.
+  nterm_ind t as [v|f ind|op bs ind] Case; simpl; auto.
+  rewrite flat_map_map; unfold compose.
+  unfold vars2sovars.
+  rewrite map_flat_map; unfold compose.
+  apply eq_flat_maps; introv i.
+  destruct x as [vs t]; simpl.
+  rewrite (ind t vs); auto.
+  unfold remove_so_vars.
+  unfold vars2sovars.
+  rewrite <- (map_diff_commute deq_nvar); eauto 2 with slow.
+Qed.
+Hint Rewrite @so_free_vars_nterm2soterm : slow.
+
+(* !!MOVE *)
+Lemma get_utokens_so_nterm2soterm {o} :
+  forall (t : @NTerm o),
+    get_utokens_so (nterm2soterm t) = get_utokens t.
+Proof.
+  nterm_ind t as [v|f ind|op bs ind] Case; simpl; auto.
+  f_equal.
+  rewrite flat_map_map; unfold compose.
+  apply eq_flat_maps; introv i.
+  destruct x as [vs t]; simpl.
+  eapply ind; eauto.
+Qed.
+Hint Rewrite @get_utokens_so_nterm2soterm : slow.
+
+Definition valid_extract {o} (t : @NTerm o) : Prop :=
+  wf_term t # closed t # noutokens t.
+
+Lemma extract2correct {o} :
+  forall (name : opname)
+         (t    : @NTerm o)
+         (v    : valid_extract t),
+    correct_abs (opname2opabs name) [] (nterm2soterm t).
+Proof.
+  introv valid.
+  destruct valid as [w v]; destruct v as [c n].
+  unfold correct_abs; simpl.
+  dands.
+  - unfold wf_soterm.
+    rewrite soterm2nterm_nterm2soterm; auto.
+  - unfold socovered; simpl.
+    rewrite so_free_vars_nterm2soterm.
+    rewrite c; simpl; auto.
+  - constructor.
+  - unfold no_utokens.
+    rewrite get_utokens_so_nterm2soterm.
+    rewrite n; auto.
+Qed.
+
+Definition extract2def {o}
+           (name  : LemmaName)
+           (ext   : @NTerm o)
+           (valid : valid_extract ext) : library_entry :=
+  lib_abs
+    (opname2opabs name)
+    []
+    (nterm2soterm ext)
+    (extract2correct name ext valid).
+
+Inductive DepLibrary {o} : @ProofContext o -> Type :=
+| DepLibrary_Empty :
+    DepLibrary (MkProofContext o [] [])
+| DepLibrary_Abs :
+    forall {ctxt}
+           (c : DepLibrary ctxt)
+           (e : @library_entry o)
+           (n : entry_not_in_lib e ctxt),
+      DepLibrary (updLibProofContext ctxt e)
+| DepLibrary_Proof :
+    forall {ctxt}
+           (c     : DepLibrary ctxt)
+           (name  : LemmaName)
+           (stmt  : @NTerm o)
+           (ext   : NTerm)
+           (valid : valid_extract ext)
+           (p     : proof ctxt (Statement stmt ext))
+           (n     : name_not_in_lib name ctxt),
+      DepLibrary (updLibProofContext
+                    (updConclProofContext ctxt (mk_concl stmt ext))
+                    (extract2def name ext valid)).
+
+Inductive LibraryEntry {o} :=
+| LibraryEntry_abs (e : @library_entry o)
+| LibraryEntry_proof
+    (ctxt  : @ProofContext o)
+    (name  : LemmaName)
+    (stmt  : NTerm)
+    (ext   : NTerm)
+    (valid : valid_extract ext)
+    (prf   : proof ctxt (Statement stmt ext)).
+
+(* A library is just a list of entries such that we store the most recent
+   entry at the front of the list
+ *)
+Definition Library {o} := list (@LibraryEntry o).
+
+Definition extend_proof_context {o} (ctxt : @ProofContext o) (e : LibraryEntry) : ProofContext :=
+  match e with
+  | LibraryEntry_abs e => updLibProofContext ctxt e
+  | LibraryEntry_proof c name stmt ext valid prf =>
+    updLibProofContext
+      (updConclProofContext ctxt (mk_concl stmt ext))
+      (extract2def name ext valid)
+  end.
+
+Definition ValidLibraryEntry {o} (ctxt : @ProofContext o) (e : LibraryEntry) : Type :=
+  match e with
+  | LibraryEntry_abs e => entry_not_in_lib e ctxt
+  | LibraryEntry_proof c name stmt ext valid prf =>
+    c = ctxt # name_not_in_lib name ctxt
+  end.
+
+Fixpoint Library2ProofContext {o} (L : @Library o) : ProofContext :=
+  match L with
+  | [] => EMPC
+  | entry :: entries =>
+    let ctxt := Library2ProofContext entries in
+    extend_proof_context ctxt entry
+  end.
+
+Fixpoint ValidLibrary {o} (L : @Library o) : Type :=
+  match L with
+  | [] => True
+  | entry :: entries =>
+    ValidLibraryEntry (Library2ProofContext entries) entry
+    # ValidLibrary entries
+  end.
+
+Definition lemma_in_LibraryEntry {o}
+           (s : @baresequent o)
+           (e : LibraryEntry) : Type :=
+  match e with
+  | LibraryEntry_abs e => False
+  | LibraryEntry_proof c name stmt ext valid prf =>
+    s = mk_baresequent [] (mk_concl stmt ext)
+  end.
+
+Fixpoint lemma_in_Library {o}
+         (s : @baresequent o)
+         (l : Library) : Type :=
+  match l with
+  | [] => False
+  | entry :: entries =>
+    lemma_in_LibraryEntry s entry
+    [+]
+    lemma_in_Library s entries
+  end.
+
+Definition seq_in_context {o}
+           (s  : @baresequent o)
+           (pc : ProofContext) : Type :=
+  {c : conclusion & s = mk_bseq [] c # LIn c (PC_conclusions pc)}.
+
+(*Lemma correct_library {o} :
+  forall {c : ProofContext} (l : Library c) (s : @baresequent o),
+    lemma_in_Library s l
+    -> sequent_true_ext_lib_wf c s.
+Proof.
+  induction l; simpl; introv i; tcsp.
+
+  - apply IHl in i; clear IHl.
+    apply sequent_true_mono_lib; auto.
+
+  - repndors.
+
+    + apply IHl in i; clear IHl.
+      apply sequent_true_mono_lib; auto.
+
+    + subst.
+
+      assert (forall c,
+                 LIn c (PC_conclusions ctxt)
+                 -> sequent_true_ext_lib_wf ctxt (mk_bseq [] c)) as imp.
+      {
+        introv i.
+        apply IHl.
+      }
+Qed.*)
+
+
+Lemma correct_library {o} :
+  forall (pc : ProofContext) (L : Library) (s : @baresequent o),
+    ValidLibrary pc L
+    -> lemma_in_Library s L
+    -> sequent_true_ext_lib_wf pc s.
+Proof.
+  induction L; introv valid i; simpl in *; tcsp.
+  repnd; repndors.
+
+  - destruct a; simpl in *; tcsp.
+    repnd; subst; simpl in *.
+
+
+
+    Focus 2.
+  apply (IHL _ s) in valid; auto.
+
+  XXXXXXXXXX
+
+  - apply IHL in i.
+    apply sequent_true_mono_lib; auto.
+
+  - repndors; subst.
+
+    +
+
+Qed.
+
+Definition pre_proofs {o} (ctxt : @ProofContext o) :=
+  list {s : pre_baresequent & pre_proof ctxt s}.
+
+Record NuprlState {o} :=
+  MkNuprlState
+    {
+      NuprlState_context    : @ProofContext o;
+      NuprlState_lib        : Library NuprlState_context;
+      NuprlState_unfinished : pre_proofs NuprlState_context;
+    }.
+
+
+
+(* ===========================================================
+
+  Commands to manipulate the state
+
+  ============================================================ *)
+
+Definition address := list nat.
+
+Inductive command {o} :=
+(* add a definition at the head *)
+| COM_add_def
+    (opabs   : opabs)
+    (vars    : list sovar_sig)
+    (rhs     : @SOTerm o)
+    (correct : correct_abs opabs vars rhs)
+(* tries to complete a proof if it has no holes *)
+| COM_finish_proof (name : LemmaName)
+(* focuses to a node in a proof *)
+| COM_focus_proof (name : LemmaName) (adr : address).
+
+Definition update {o}
+           (state : @NuprlState o)
+           (com   : command) : NuprlState :=
+  match com with
+  | COM_add_def opabs vars rhs correct =>
+    NuprlState_add_def_lib state opabs vars rhs correct
+  | COM_finish_proof name =>
+    let lib := NuprlState_proof_library state in
+    NuprlState_upd_proof_lib state (finish_proof_in_library lib name)
+  | COM_focus_proof name addr =>
+    let lib := NuprlState_proof_library state in
+    NuprlState_upd_focus state (focus_proof_in_library lib name addr)
+  end.
